src/axiomatic/Machine.v
@@ -51,12 +51,14 @@ Inductive mstep mc mc' e i : Prop :=
       (TIDa: thread a = i) 
       (GSTEP: gstep (acts mc) (sb mc) (rmw mc) (rf mc) (mo mc) (sc mc)
                     (acts mc') (sb mc') (rmw mc') (rf mc') (mo mc') (sc mc') a)
+      (COH': Coherent (acts mc') (sb mc') (rmw mc') (rf mc') (mo mc') (sc mc'))
   | write a l v o 
       (EVENT: e = Some (ProgramEvent.write l v o)) 
       (LABa: lab a = Astore l v o) 
       (TIDa: thread a = i) 
       (GSTEP: gstep (acts mc) (sb mc) (rmw mc) (rf mc) (mo mc) (sc mc)
                     (acts mc') (sb mc') (rmw mc') (rf mc') (mo mc') (sc mc') a)
+      (COH': Coherent (acts mc') (sb mc') (rmw mc') (rf mc') (mo mc') (sc mc'))
   | update a_r a_w l v_r v_w o_r o_w 
       (EVENT: e = Some (ProgramEvent.update l v_r v_w o_r o_w)) 
       (LABar: lab a_r = Aload l v_r o_r) (LABaw: lab a_w = Astore l v_w o_w) 
@@ -66,11 +68,15 @@ Inductive mstep mc mc' e i : Prop :=
            (acts mc_mid) (sb mc_mid) (rmw mc_mid) (rf mc_mid) (mo mc_mid) (sc mc_mid) a_r)
       (GSTEPw: gstep (acts mc_mid) (sb mc_mid) (rmw mc_mid) (rf mc_mid) (mo mc_mid) (sc mc_mid)
                      (acts mc') (sb mc') (rmw mc') (rf mc') (mo mc') (sc mc') a_w)
+      (COHmid: Coherent (acts mc_mid) (sb mc_mid) (rmw mc_mid) (rf mc_mid) (mo mc_mid) 
+                        (sc mc_mid))
+      (COH': Coherent (acts mc') (sb mc') (rmw mc') (rf mc') (mo mc') (sc mc'))
   | fence a o_r o_w (EVENT: e = Some (ProgramEvent.fence o_r o_w)) 
       (LABa: lab a = Afence o_r o_w) 
       (TIDa: thread a = i) 
       (GSTEP: gstep (acts mc) (sb mc) (rmw mc) (rf mc) (mo mc) (sc mc)
-                    (acts mc') (sb mc') (rmw mc') (rf mc') (mo mc') (sc mc') a).
+                    (acts mc') (sb mc') (rmw mc') (rf mc') (mo mc') (sc mc') a)
+      (COH': Coherent (acts mc') (sb mc') (rmw mc') (rf mc') (mo mc') (sc mc')).
 
 Inductive step mc mc' : Prop :=
 | step_intro  
